SortedList.lean
@@ -1,3 +1,4 @@
 -- This module serves as the root of the `SortedList` library.
 -- Import modules here that should be built as part of the library.
-import SortedList.SortedList
+import SortedList.Recursive
+import SortedList.Imperative
