SortedList/Specification.lean
@@ -1,0 +1,14 @@
+import SortedList.Basic
+
+open List
+
+/-- The key properties that a `unique` function must have together defines its specification. -/
+structure UniqueSpec (unique : List Int → List Int) where
+  /-- Every element in the input is in the output -/
+  supset : ∀ l, l ⊆ unique l
+  /-- Every element in the output is in the input -/
+  subset : ∀ l, unique l ⊆ l
+  /-- The output is sorted if the input is sorted -/
+  sorted_if_sorted : ∀ l, (Sorted l) → Sorted (unique l)
+  /-- The output contains no duplicates if the input is sorted -/
+  nodup_if_sorted : ∀ l, (Sorted l) → Nodup (unique l)
